Fifo/Proofs1.v
@@ -1,0 +1,163 @@
+Require Import Kami.Lib.EclecticLib.
+Require Import Kami.All.
+Require Import Kami.GallinaModules.Relations.
+Require Import Kami.GallinaModules.AuxLemmas.
+Require Import Kami.GallinaModules.AuxTactics.
+Require Import StdLibKami.RegArray.CorrectDef.
+Require Import StdLibKami.Fifo.Ifc.
+Require Import StdLibKami.Fifo.Impl.
+Require Import StdLibKami.Fifo.Spec.
+Require Import StdLibKami.Fifo.CorrectDef.
+
+Section Proofs1.
+  Context {ifcParams' : Fifo.Ifc.Params}.
+  Variable Hsize1 : size = 1.
+  Variable impl1Params impl2Params : Impl.Params.
+  Local Definition fifoImpl1 := @Fifo.Impl.impl ifcParams' impl1Params.
+  Local Definition fifoImpl2 := @Fifo.Impl.impl ifcParams' impl2Params.
+
+  Record myFifoImpl1R  (implRegs : RegsT) (fifo1_bval : bool) (fifo1_dval : type k)
+         (o_i o_s : RegsT) : Prop :=
+    {
+      implRegVal : implRegs = [(Fifo1.validRegName,
+                                existT _ (SyntaxKind Bool) fifo1_bval);
+                              (Fifo1.dataRegName,
+                               existT _ (SyntaxKind k) fifo1_dval)];
+      Ho_iCorrect1 : o_i = implRegs;
+      Ho_sCorrect1 : o_s = implRegs;
+      Ho_iNoDup1 : NoDup (map fst o_i);
+      Ho_sNoDup1 : NoDup (map fst o_s);
+    }.
+
+  Ltac Record_destruct :=
+    match goal with
+    |[ H : exists _ _ _, myFifoImpl1R _ _ _ _ _ |- _] =>
+     let implRegs := fresh "implRegs" in
+     let fifo1_bval := fresh "fifo1_bval" in
+     let fifo1_dval := fresh "fifo1_dval" in
+     let H0 := fresh "H" in
+     destruct H as [implRegs [fifo1_bval [fifo1_dval H0]]]; destruct H0
+    end.
+
+  Goal FifoCorrect fifoImpl1 fifoImpl2.
+    rewrite <- Nat.eqb_eq in Hsize1.
+    all : econstructor 1 with (fifoR := (fun o1 o2 =>
+                                           (exists implRegs fifo1_bval fifo1_dval,
+                                               myFifoImpl1R implRegs
+                                                            fifo1_bval fifo1_dval o1 o2)))
+                              (fifoRegs := [(Fifo1.validRegName,
+                                             SyntaxKind Bool);
+                                            (Fifo1.dataRegName,
+                                             SyntaxKind k)]).
+    all : red; unfold fifoImpl1, fifoImpl2, impl, spec, regArray,
+               isEmpty, flush, enq, deq, numFree, isFull, first,
+               Impl.isEmpty, Impl.flush, Impl.enq, Impl.deq, Impl.numFree,
+               Impl.isFull, Impl.first.
+    all : try rewrite Hsize1; unfold Fifo1.impl, Fifo1.isEmpty,
+                         Fifo1.isFull, Fifo1.flush, Fifo1.numFree, Fifo1.first,
+                         Fifo1.deq, Fifo1.enq; intros; try Record_destruct.
+    - hyp_consumer; goal_consumer1.
+    - hyp_consumer; goal_consumer2; eauto.
+    - hyp_consumer; goal_consumer1.
+    - hyp_consumer; goal_consumer2; eauto.
+    - hyp_consumer; goal_consumer1.
+    - hyp_consumer; goal_consumer2; eauto.
+    - hyp_consumer; goal_consumer1.
+    - hyp_consumer; goal_consumer2.
+    - hyp_consumer; goal_consumer1.
+      econstructor; repeat normal_solver; repeat my_risky_solver.
+    - hyp_consumer; goal_consumer2.
+    - hyp_consumer; goal_consumer1.
+      econstructor; repeat normal_solver; repeat my_risky_solver.
+    - hyp_consumer; goal_consumer2.
+    - hyp_consumer; goal_consumer1.
+      econstructor; repeat normal_solver; repeat my_risky_solver.
+    - hyp_consumer; goal_consumer2; eauto.
+  Qed.
+End Proofs1.
+
+Section Proofs2.
+  Context {ifcParams' : Fifo.Ifc.Params}.
+  Variable Hsize1 : size <> 1.
+  Variable impl1Params impl2Params : Impl.Params.
+  Local Definition regArray1 := @regArray ifcParams' impl1Params.
+  Local Definition regArray2 := @regArray ifcParams' impl2Params.
+  Local Definition fifoImpl1' := @Fifo.Impl.impl ifcParams' impl1Params.
+  Local Definition fifoImpl2' := @Fifo.Impl.impl ifcParams' impl2Params.
+  
+  Variable HRegArrayCorrect : RegArrayCorrect regArray1 regArray2.
+
+  Record myFifoImplR (regArrayR : RegsT -> RegsT -> Prop) regArrayRegs
+         (implRegs : RegsT) (enqVal deqVal : word (Fifo.Ifc.lgSize + 1))
+         (regArray1Regs regArray2Regs : RegsT) (o_i o_s : RegsT) : Prop :=
+    {
+      implRegVal' : implRegs = [(Fifo.Impl.deqPtrName,
+                                existT _ (SyntaxKind (Bit (Fifo.Ifc.lgSize + 1))) deqVal);
+                              (Fifo.Impl.enqPtrName,
+                               existT _ (SyntaxKind (Bit (Fifo.Ifc.lgSize + 1))) enqVal)];
+      Ho_iCorrect : o_i = implRegs ++ regArray1Regs;
+      Ho_sCorrect : o_s = implRegs ++ regArray2Regs;
+      Ho_iNoDup : NoDup (map fst o_i);
+      Ho_sNoDup : NoDup (map fst o_s);
+      HRegArrayRegs : getKindAttr regArray1Regs = regArrayRegs;
+      HRegArray : regArrayR regArray1Regs regArray2Regs;
+    }.
+  
+  Ltac Record_destruct :=
+    match goal with
+    |[ H : exists _ _ _ _ _, myFifoImplR _ _ _ _ _ _ _ _ _ |- _] =>
+     let implRegs := fresh "implRegs" in
+     let enqVal := fresh "enqVal" in
+     let deqVal := fresh "deqVal" in
+     let regArray1Regs := fresh "regArray1Regs" in
+     let regArray2Regs := fresh "regArray2Regs" in
+     let H0 := fresh "H" in
+     destruct H as [implRegs [enqVal [deqVal [regArray1Regs [regArray2Regs H0]]]]];
+     destruct H0
+    end.
+
+  Goal FifoCorrect fifoImpl1' fifoImpl2'.
+    destruct HRegArrayCorrect.
+    rewrite <- Nat.eqb_neq in Hsize1.
+    all : econstructor 1 with (fifoR := (fun o1 o2 =>
+                                           (exists implRegs enqVal deqVal
+                                                  regArray1Regs regArray2Regs,
+                                               myFifoImplR regArrayR regArrayRegs implRegs
+                                                           enqVal deqVal
+                                                           regArray1Regs regArray2Regs o1 o2)))
+                        (fifoRegs := [(Fifo.Impl.deqPtrName,
+                                       (SyntaxKind (Bit (Fifo.Ifc.lgSize + 1))));
+                                      (Fifo.Impl.enqPtrName,
+                                       (SyntaxKind (Bit (Fifo.Ifc.lgSize + 1))))]
+                                       ++ regArrayRegs).
+    all : red; unfold fifoImpl1', fifoImpl2', impl, spec, regArray,
+               isEmpty, flush, enq, deq, numFree, isFull, first,
+               Impl.isEmpty, Impl.flush, Impl.enq, Impl.deq, Impl.numFree,
+               Impl.isFull, Impl.first.
+    all : try rewrite Hsize1; unfold Fifo1.impl, Fifo1.isEmpty,
+                         Fifo1.isFull, Fifo1.flush, Fifo1.numFree, Fifo1.first,
+                         Fifo1.deq, Fifo1.enq; intros; try Record_destruct.
+    all : unfold regArray1, Impl.isEmpty in *.
+    - hyp_consumer; goal_consumer1.
+    - hyp_consumer; goal_consumer2.
+    - hyp_consumer; goal_consumer1.
+    - hyp_consumer; goal_consumer2.
+    - hyp_consumer; goal_consumer1.
+    - hyp_consumer; goal_consumer2.
+    - hyp_consumer; goal_consumer1.
+    - hyp_consumer; goal_consumer2; goal_consumer1.
+    - hyp_consumer; goal_consumer1.
+      econstructor; eauto; normalize_key_concl.
+    - hyp_consumer; goal_consumer2; goal_consumer1.
+    - hyp_consumer; goal_consumer1; econstructor; eauto; normalize_key_concl;
+      repeat rewrite doUpdRegs_preserves_keys; normalize_key_concl.
+      gka_doUpdReg_red; normal_solver; auto.
+    - hyp_consumer; goal_consumer2; goal_consumer1.
+    - hyp_consumer; goal_consumer1.
+      econstructor; eauto; normalize_key_concl.
+    - hyp_consumer; goal_consumer2; eauto.
+      Unshelve.
+      all : eauto; try exact nil; try exact WO.
+  Qed.
+  
+End Proofs2.
