RegArray/CorrectDef.v
@@ -1,0 +1,23 @@
+Require Import Kami.All.
+Require Import StdLibKami.RegArray.Impl.
+Require Import StdLibKami.RegArray.Ifc.
+Require Import StdLibKami.RegArray.Spec.
+Require Import Kami.GallinaModules.AuxLemmas.
+Require Import Kami.GallinaModules.AuxTactics.
+Require Import Kami.GallinaModules.Relations.
+Require Import Coq.Logic.EqdepFacts.
+
+Section CorrectDef.
+  
+  Context `{Params : RegArray.Ifc.Params}.
+  Record RegArrayCorrect (imp spec: RegArray.Ifc.Ifc): Type :=
+    {
+      regArrayRegs : list (Attribute FullKind);
+      regArrayR : RegsT -> RegsT -> Prop;
+      readCorrect : forall idx, EffectlessRelation regArrayR (@read _ imp type idx)
+                                                   (@read _ spec type idx);
+      readWb : forall idx, ActionWb regArrayRegs (@read _ imp type idx);
+      writeCorrect : forall val, EffectfulRelation regArrayR (@write _ imp type val) (@write _ spec type val);
+      writeWb : forall val, ActionWb regArrayRegs (@write _ imp type val);
+    }.
+End CorrectDef.
