RegArray/Proofs.v
@@ -1,11 +1,12 @@
+Require Import Coq.Logic.EqdepFacts.
 Require Import Kami.All.
-Require Import StdLibKami.RegArray.Impl.
-Require Import StdLibKami.RegArray.Ifc.
-Require Import StdLibKami.RegArray.Spec.
 Require Import Kami.GallinaModules.AuxLemmas.
 Require Import Kami.GallinaModules.AuxTactics.
 Require Import Kami.GallinaModules.Relations.
-Require Import Coq.Logic.EqdepFacts.
+Require Import StdLibKami.RegArray.Impl.
+Require Import StdLibKami.RegArray.Ifc.
+Require Import StdLibKami.RegArray.Spec.
+Require Import StdLibKami.RegArray.CorrectDef.
 
 Definition SemAction_le {k} (a1 a2 : ActionT type k) :=
   forall o reads upds calls retV,
@@ -1359,16 +1360,6 @@ Qed.
 
 Section Proofs.
   Context `{Params : RegArray.Ifc.Params}.
-  Record RegArrayCorrect (imp spec: RegArray.Ifc.Ifc): Type :=
-  {
-    regArrayRegs : list (Attribute FullKind);
-    regArrayR : RegsT -> RegsT -> Prop;
-    readCorrect : forall idx, EffectlessRelation regArrayR (@read _ imp type idx)
-                                                 (@read _ spec type idx);
-    readWb : forall idx, ActionWb regArrayRegs (@read _ imp type idx);
-    writeCorrect : forall val, EffectfulRelation regArrayR (@write _ imp type val) (@write _ spec type val);
-    writeWb : forall val, ActionWb regArrayRegs (@write _ imp type val);
-  }.
 
   Local Notation Idx := (Bit (Nat.log2_up size)).
   Definition implRegArray := @Impl.impl Params.
